src/PlutusIR/Analysis/NoShadow.v
@@ -1,0 +1,293 @@
+From PlutusCert Require Import
+  PlutusIR
+  Analysis.BoundVars
+  Analysis.FreeVars
+  Util.List
+.
+
+Require Import
+  Strings.String
+  Lists.List
+.
+Import Utf8_core.
+Import ListNotations.
+
+(*
+Note [No Shadowing]
+-------------------
+A term has shadowing when it binds a variable that is already in scope. To avoid this,
+we keep track of the variables in scope (ctx), and at every binding site, check if the
+name was not already bound.
+
+*)
+
+(* A context is used to track the names of variables, so we can avoid shadowing *)
+Definition ctx := list string.
+
+Reserved Notation "Δ '|-*ns' T" (at level 40, T at level 0).
+Inductive no_shadow_ty (Δ : ctx) : ty -> Prop :=
+  | NS_Ty_Forall : forall X K T,
+      X ∉ Δ ->
+      (X :: Δ) |-*ns T ->
+      Δ |-*ns (Ty_Forall X K T)
+  | NS_Ty_Lam : forall X K1 T,
+      X ∉ Δ ->
+      (X :: Δ) |-*ns T ->
+      Δ |-*ns (Ty_Lam X K1 T)
+
+  | NS_Ty_Var : forall X,
+      In X Δ ->
+      Δ |-*ns (Ty_Var X)
+  | NS_Ty_Fun : forall T1 T2,
+      Δ |-*ns T1 ->
+      Δ |-*ns T2 ->
+      Δ |-*ns (Ty_Fun T1 T2)
+  | NS_Ty_IFix  : forall F T,
+      Δ |-*ns T ->
+      Δ |-*ns F ->
+      Δ |-*ns (Ty_IFix F T)
+  | NS_Ty_Builtin : forall T,
+      Δ |-*ns (Ty_Builtin T)
+  | NS_Ty_App : forall T1 T2,
+      Δ |-*ns T1 ->
+      Δ |-*ns T2 ->
+      Δ |-*ns (Ty_App T1 T2)
+where "Δ '|-*ns' T " := (no_shadow_ty Δ T).
+
+Reserved Notation "Δ ',,' Γ '|-+ns' t " (at level 101, t at level 0, no associativity).
+Reserved Notation "Δ '|-ns_ok_c' c " (at level 101, c at level 0).
+Reserved Notation "Δ ',,' Γ  '|-ns_oks_nr' bs" (at level 101, bs at level 0, no associativity).
+Reserved Notation "Δ ',,' Γ '|-ns_oks_r' bs" (at level 101, bs at level 0, no associativity).
+Reserved Notation "Δ ',,' Γ '|-ns_ok_b' b" (at level 101, b at level 0, no associativity).
+
+Inductive no_shadow : ctx -> ctx -> term -> Prop :=
+  | NS_LamAbs : forall Δ Γ x T t,
+      x ∉ Γ ->
+      Δ |-*ns T ->
+      Δ ,, (x :: Γ) |-+ns t ->
+      Δ ,, Γ |-+ns (LamAbs x T t)
+  | NS_TyAbs : forall Δ Γ X K t,
+      X ∉ Δ ->
+      (X :: Δ) ,, Γ |-+ns t ->
+      Δ ,, Γ |-+ns (TyAbs X K t)
+
+  | NS_Var : forall Δ Γ x,
+      In x Γ ->
+      Δ ,, Γ |-+ns (Var x)
+  | NS_Apply : forall Δ Γ t1 t2,
+      Δ ,, Γ |-+ns t1 ->
+      Δ ,, Γ |-+ns t2 ->
+      Δ ,, Γ |-+ns (Apply t1 t2)
+  | NS_TyInst : forall Δ Γ t T,
+      Δ ,, Γ |-+ns t ->
+      Δ |-*ns T ->
+      Δ ,, Γ |-+ns (TyInst t T)
+  | NS_IWrap : forall Δ Γ F T M,
+      Δ |-*ns F ->
+      Δ |-*ns T ->
+      Δ ,, Γ |-+ns M ->
+      Δ ,, Γ |-+ns (IWrap F T M)
+  | NS_Unwrap : forall Δ Γ M,
+      Δ ,, Γ |-+ns M ->
+      Δ ,, Γ |-+ns (Unwrap M)
+  | NS_Constant : forall Δ Γ (c : constant),
+      Δ ,, Γ |-+ns (Constant c)
+  | NS_Builtin : forall Δ Γ f,
+      Δ ,, Γ |-+ns (Builtin f)
+  | NS_Error : forall Δ Γ S,
+      Δ |-*ns S ->
+      Δ ,, Γ |-+ns (Error S)
+
+  | NS_Let : forall Δ Γ bs t Δ_bs Γ_bs,
+      Δ_bs = rev (btvbs bs) ->
+      Γ_bs = rev (bvbs bs) ->
+      Δ ,, Γ |-ns_oks_nr bs ->
+      (Δ_bs ++ Δ) ,, (Γ_bs ++ Γ) |-+ns t ->
+      Δ ,, Γ |-+ns (Let NonRec bs t)
+
+  | NS_LetRec : forall Δ Γ bs t Δ_bs Γ_bs,
+      Δ_bs = rev (btvbs bs) ->
+      Γ_bs = rev (bvbs bs) ->
+      Forall (fun X => X ∉ Δ) Δ_bs ->
+      Forall (fun x => x ∉ Γ) Δ_bs ->
+      NoDup Δ_bs ->
+      NoDup Γ_bs ->
+      (Δ_bs ++ Δ) ,, (Γ_bs ++ Γ) |-ns_oks_r bs ->
+      (Δ_bs ++ Δ) ,, (Γ_bs ++ Γ) |-+ns t ->
+      Δ ,, Γ |-+ns (Let Rec bs t)
+
+
+with ns_bindings_nonrec : ctx -> ctx -> list binding -> Prop :=
+
+  | NS_NilB_NonRec : forall Δ Γ,
+    Δ ,, Γ |-ns_oks_nr nil
+
+  | NS_ConsB_NonRec : forall Δ Γ b bs,
+      Forall (fun X => X ∉ Δ) (btvb b) ->
+      Forall (fun x => x ∉ Δ) (bvb b) ->
+      Δ ,, Γ |-ns_ok_b b ->
+      (btvb b ++ Δ) ,, (bvb b ++ Γ) |-ns_oks_nr bs ->
+      Δ ,, Γ |-ns_oks_nr (b :: bs)
+
+with ns_bindings_rec : ctx -> ctx -> list binding -> Prop :=
+
+  | NS_NilB_Rec : forall Δ Γ,
+      Δ ,, Γ |-ns_oks_r nil
+  | NS_ConsB_Rec : forall Δ Γ b bs,
+      Δ ,, Γ |-ns_ok_b b ->
+      Δ ,, Γ |-ns_oks_r bs ->
+      Δ ,, Γ |-ns_oks_r (b :: bs)
+
+with ns_binding : ctx -> ctx -> binding -> Prop :=
+  | NS_TermBind : forall Δ Γ s x T t,
+      Δ |-*ns T ->
+      Δ ,, Γ |-+ns t ->
+      Δ ,, Γ |-ns_ok_b (TermBind s (VarDecl x T) t)
+  | NS_TypeBind : forall Δ Γ X K T,
+      Δ |-*ns T ->
+      Δ ,, Γ |-ns_ok_b (TypeBind (TyVarDecl X K) T)
+  | NS_DataBind : forall Δ Γ X YKs cs matchFunc Δ',
+      Δ' = rev (map tvdecl_name YKs) ++ Δ  ->
+      (forall c, In c cs -> Δ' |-ns_ok_c c) ->
+      Δ ,, Γ |-ns_ok_b (DatatypeBind (Datatype X YKs matchFunc cs))
+
+with constructor_well_formed : ctx -> vdecl -> Prop :=
+  | NS_Con : forall Δ x T,
+      Δ |-*ns T ->
+      Δ |-ns_ok_c (VarDecl x T)
+  where "Δ '|-ns_ok_c' c" := (constructor_well_formed Δ c)
+  and "Δ ',,' Γ '|-+ns' t" := (no_shadow Δ Γ t)
+  and "Δ ',,' Γ '|-ns_oks_nr' bs" := (ns_bindings_nonrec Δ Γ bs)
+  and "Δ ',,' Γ '|-ns_oks_r' bs" := (ns_bindings_rec Δ Γ bs)
+  and "Δ ',,' Γ '|-ns_ok_b' b" := (ns_binding Δ Γ b)
+.
+
+
+Scheme no_shadow__ind := Minimality for no_shadow Sort Prop
+  with ns_bindings_nonrec__ind := Minimality for ns_bindings_nonrec Sort Prop
+  with ns_bindings_rec__ind := Minimality for ns_bindings_rec Sort Prop
+  with ns_binding__ind := Minimality for ns_binding Sort Prop
+.
+
+Combined Scheme no_shadow__multind from
+  no_shadow__ind,
+  ns_bindings_nonrec__ind,
+  ns_bindings_rec__ind,
+  ns_binding__ind
+.
+
+Definition multind P_ns P_ns_nonrec P_ns_rec P_ns_bind :=
+  (∀ Δ Γ t, no_shadow Δ Γ t -> P_ns Δ Γ t) /\
+  (∀ Δ Γ bs, ns_bindings_nonrec Δ Γ bs -> P_ns_nonrec Δ Γ bs) /\
+  (∀ Δ Γ bs, ns_bindings_rec Δ Γ bs -> P_ns_rec Δ Γ bs) /\
+  (∀ Δ Γ b, ns_binding Δ Γ b -> P_ns_bind Δ Γ b)
+.
+
+
+Definition closed := no_shadow [] [].
+
+
+
+Module Ty.
+
+  Import FreeVars.Ty.
+  Import BoundVars.Ty.
+
+  (* TODO: move to Util.List *)
+  Notation "xs ⊑ ys" := (incl xs ys) (at level 70, no associativity).
+
+  (* TODO: move to Util.List *)
+  Lemma remove_incl {A} xs ys f (x : A) :
+    xs ⊑ (x :: ys) -> remove f x xs ⊑ ys.
+  Proof.
+  Admitted.
+
+  Create HintDb incl.
+  Hint Resolve remove_incl incl_nil_l incl_cons incl_app
+    : incl.
+
+  Lemma ns_ftv Δ T : no_shadow_ty Δ T -> ftv T ⊑ Δ.
+  Proof.
+    induction 1; rewrite ftv_equation; auto with incl.
+  Qed.
+
+  Create HintDb disjoint.
+  Hint Resolve disjoint_cons_r disjoint_cons_l disjoint_nil_l disjoint_nil_r
+    disjoint_app_r disjoint_app_l
+    : disjoint.
+
+  Hint Resolve disjoint_uncons_r disjoint_uncons_l | 10 (* higher cost to prevent useless identities *)
+    : disjoint.
+
+  Lemma ns_disjoint Δ T : no_shadow_ty Δ T -> disjoint Δ (btv T).
+  Proof.
+    induction 1; rewrite btv_equation; eauto with disjoint.
+  Qed.
+
+End Ty.
+
+
+Module Term.
+
+(* TODO: move to Util.List *)
+Notation "xs ⊑ ys" := (incl xs ys) (at level 70, no associativity).
+
+
+Definition ctx_bound__term (Δ Γ : ctx) t :=
+  (∀ x, x ∈ Γ -> x ∉ bound_vars t) /\
+  (∀ X, X ∈ Δ -> X ∉ btv t).
+
+(* reused for let and letrec: bound_vars and btv make no distinction between recursive and non-recursive lets *)
+Definition ctx_bound__let (Δ Γ : ctx) bs := 
+  (∀ x, x ∈ Γ -> x ∉ concat (map bound_vars_binding bs)) /\
+  (∀ X, X ∈ Δ -> X ∉ concat (map btv_binding bs)).
+
+Definition ctx_bound__bind (Δ Γ : ctx) b := 
+  (∀ x, x ∈ Γ -> x ∉ bound_vars_binding b) /\
+  (∀ x, x ∈ Δ -> x ∉ btv_binding b).
+
+Lemma no_shadow__ctx_bound : multind ctx_bound__term ctx_bound__let ctx_bound__let ctx_bound__bind.
+  apply no_shadow__multind.
+  - unfold ctx_bound__term. intros.
+    split.
+    + intros y H_y_in.
+      destruct H2 as [IH1 _].
+      specialize (IH1 y).
+      assert (y ∉ bound_vars t) by intuition.
+      assert (x <> y). { destruct (string_dec x y); try assumption. subst x. contradiction. }
+      simpl.
+      intuition.
+      (* etc. *)
+Admitted.
+
+
+(*
+(* Corollaries that play nice with auto *)
+Corollary ns_ctx Δ Γ t :
+  no_shadow Δ Γ t ->
+  (∀ x, x ∈ Γ -> x ∉ bound_vars t) /\
+  (∀ X, X ∈ Δ -> X ∉ btv t).
+Proof.
+  apply no_shadow__ctx_bound.
+Qed.
+
+Corollary ns_tctx Δ Γ t :
+  no_shadow Δ Γ t ->
+  (∀ x, x ∈ Γ -> x ∉ bound_vars t).
+Proof.
+  apply ns_ctx.
+Qed.
+*)
+
+
+  Lemma ns_disjoint_ann Δ Γ t : no_shadow Δ Γ t -> disjoint Δ (btv t).
+  Proof.
+  Admitted.
+
+
+  Lemma ns_disjoint Δ Γ t : no_shadow Δ Γ t -> disjoint Γ (bound_vars t).
+  Proof.
+  Admitted.
+
+End Term.
+
